semtyping.v
@@ -1,195 +1,263 @@
-From WR Require Import syntax join imports.
-
-Definition SBool (a : tm) := exists v, Pars a v /\ (is_bool_val v \/ ne v).
-Definition SUniv (I : nat -> tm -> (tm -> Prop) -> Prop) m A := exists PA, I m A PA.
-Definition SEq a b p := (Pars p tRefl /\ Coherent a b) \/ wne p.
+From WR Require Import syntax join normalform imports.
 
 Definition ProdSpace (PA : tm -> Prop) (PF : tm -> (tm -> Prop) -> Prop) (b : tm) :=
   forall a PB, PA a -> PF a PB -> PB (tApp b a).
 
-Inductive InterpExt n (I : nat -> tm -> (tm -> Prop) -> Prop) : tm -> (tm -> Prop) -> Prop :=
-| InterpExt_Ne A : ne A -> InterpExt n I A wne
-| InterpExt_Void : InterpExt n I tVoid wne
-| InterpExt_Bool : InterpExt n I tBool SBool
-| InterpExt_Fun A B PA (PF : tm -> (tm -> Prop) -> Prop) :
-  InterpExt n I A PA ->
+(* Logical Relation:
+
+  InterpUnivN i A P  holds when
+   - A is a Set i
+   - P is a predicate on terms that act like type A
+
+  We define this in two parts: one that generalizes over
+  smaller interpretations and then tie the knot
+  with the real definition below.
+
+ *)
+
+Reserved Notation "⟦ A ⟧ i , I ↘ S" (at level 70).
+Inductive InterpExt i (I : nat -> tm -> Prop) : tm -> (tm -> Prop) -> Prop :=
+| InterpExt_Ne A : ne A -> ⟦ A ⟧ i , I ↘ wne
+| InterpExt_Void : ⟦ tVoid ⟧ i , I ↘ wne
+| InterpExt_Bool : ⟦ tBool ⟧ i , I ↘ (fun a => exists v, a ⇒* v /\ (is_bool_val v \/ ne v))
+| InterpExt_Fun A B PA PF :
+  ⟦ A ⟧ i , I ↘ PA ->
   (forall a, PA a -> exists PB, PF a PB) ->
-  (forall a PB, PF a PB -> InterpExt n I (subst_tm (a..) B) PB) ->
-  InterpExt n I (tPi A B) (ProdSpace PA PF)
-| InterpExt_Univ m :
-  m < n ->
-  InterpExt n I (tUniv m) (SUniv I m)
+  (forall a PB, PF a PB -> ⟦ B[a..] ⟧ i , I ↘ PB) ->
+  ⟦ tPi A B ⟧ i , I ↘ (ProdSpace PA PF)
+| InterpExt_Univ j :
+  j < i ->
+  ⟦ tUniv j ⟧ i , I ↘ (I j)
 | InterpExt_Eq a b A :
   nf a ->
   nf b ->
   nf A ->
-  InterpExt n I (tEq a b A) (SEq a b)
+   ⟦ tEq a b A ⟧ i , I ↘ (fun p => (p ⇒* tRefl /\ Coherent a b) \/ wne p)
 | InterpExt_Step A A0 PA :
-  Par A A0 ->
-  InterpExt n I A0 PA ->
-  InterpExt n I A PA.
+  (A ⇒ A0) ->
+  ⟦ A0 ⟧ i , I ↘ PA ->
+  ⟦ A ⟧ i , I ↘ PA
+where "⟦ A ⟧ i , I ↘ S" := (InterpExt i I A S).
 
-Hint Constructors InterpExt : iext.
 
-Definition CR (P : tm -> Prop) :=
-  (forall a, P a -> wn a) /\
-    (forall a, wne a -> P a).
-
-Lemma ext_wn (a : tm) i :
-    wn (tApp a (var_tm i)) ->
-    wn a.
-Proof.
-  move E : (tApp a (var_tm i)) => a0 [v [hr hv]].
-  move : a E.
-  move : hv.
-  elim : a0 v / hr.
-  - hauto q:on inv:tm ctrs:rtc b:on db: nfne.
-  - move => a0 a1 a2 hr0 hr1 ih hnfa2.
-    move /(_ hnfa2) in ih.
-    move => a.
-    case : a0 hr0=>// => b0 b1.
-    elim /Par_inv=>//.
-    + hauto q:on inv:Par ctrs:rtc b:on.
-    + move => ? a0 a3 b2 b3 ? ? [? ?] ? [? ?]. subst.
-      have ? : b3 = var_tm i by hauto lq:on inv:Par. subst.
-      suff : wn (tAbs a3) by hauto lq:on unfold:wn ctrs:rtc.
-      have : wn (subst_tm ((var_tm i) ..) a3) by sfirstorder.
-      replace (subst_tm ((var_tm i) ..) a3) with (ren_tm (i..) a3).
-      move /wn_antirenaming.
-      by apply : wn_abs.
-      substify. by asimpl.
-Qed.
-
-Lemma adequacy n I (h0 : forall m, m < n -> CR (SUniv I m)) A PA
-  (h : InterpExt n I A PA)  :
-  CR PA.
-Proof.
-  elim : A PA / h=>//.
-  - firstorder with nfne.
-  - firstorder with nfne.
-  - hauto q:on db:nfne.
-  - move => A B PA PF hA ihA hTot hRes ih.
-    split.
-    + rewrite /ProdSpace => b hb.
-      have hzero : PA (var_tm var_zero) by hauto lq:on ctrs:rtc.
-      move : hTot (hzero); move/[apply]. move => [PB ?].
-      apply ext_wn with (i := var_zero).
-      hauto q:on.
-    + rewrite /ProdSpace => b wneb a PB ha hPB.
-      suff : wn a by hauto q:on use:wne_app. firstorder.
-  - hauto lq:on db:nfne.
-Qed.
-
-Lemma InterpExt_wn_ty n I A PA
-  (h0 : forall m, m < n -> CR (SUniv I m))
-  (h : InterpExt n I A PA) :
-  wn A.
-Proof.
-  elim : A PA / h; auto with nfne.
-  - move => A B PA PF hPA wnA hTot hRes ih.
-    apply wn_pi; first by auto.
-    have hzero : PA (var_tm var_zero) by hauto q:on ctrs:rtc use:adequacy.
-    move : hTot (hzero); move/[apply]. move => [PB].
-    move /ih.
-    match goal with [|- wn ?Q -> _] => replace Q with (ren_tm (var_zero..) B) end.
-    eauto using wn_antirenaming.
-    substify. by asimpl.
-  - hauto lq:on use:wn_eq ctrs:rtc.
-  - hauto lq:on ctrs:rtc.
-Qed.
-
-Lemma InterpExt_Eq' n I PA a b A :
+Lemma InterpExt_Eq' i I PA a b A :
   nf a ->
   nf b ->
   nf A ->
-  PA = SEq a b ->
-  InterpExt n I (tEq a b A) PA.
+  PA = (fun p => (p ⇒* tRefl /\ Coherent a b) \/ wne p) ->
+  ⟦ tEq a b A ⟧ i , I ↘ PA.
 Proof. hauto lq:on use:InterpExt_Eq. Qed.
 
-Lemma InterpExt_Univ' n I m PF :
-  PF = (SUniv I m) ->
-  m < n ->
-  InterpExt n I (tUniv m) PF.
+Lemma InterpExt_Univ' i I j PF :
+  PF = I j ->
+  j < i ->
+  ⟦ tUniv j ⟧ i , I ↘ PF.
 Proof. hauto lq:on ctrs:InterpExt. Qed.
 
 Equations InterpUnivN (n : nat) : tm -> (tm -> Prop) -> Prop by wf n lt :=
-  InterpUnivN n := InterpExt n (fun m A PA =>
+  InterpUnivN n := InterpExt n (fun m A =>
                                   match Compare_dec.lt_dec m n with
-                                  | left h => InterpUnivN m A PA
+                                  | left h => exists PA, InterpUnivN m A PA
                                   | right _ => False
                                   end).
 
-Lemma InterpExt_preservation n I A B P (h : InterpExt n I A P) :
-  Par A B ->
-  InterpExt n I B P.
+Notation "⟦ A ⟧ i ↘ S" := (InterpUnivN i A S) (at level 70).
+
+(* ---------------------------------------------------- *)
+
+(* The definition of InterpUnivN is more complicated than
+   it needs to be. We show that that we can
+   simplify the unfolding above to just mention InterpUnivN
+   without doing the case analysis.
+*)
+Lemma InterpExt_lt_redundant i I A PA
+  (h : ⟦ A ⟧ i , I ↘ PA) :
+       ⟦ A ⟧ i , (fun j A =>
+                     match Compare_dec.lt_dec j i with
+                     | left h => I j A
+                     | right _ => False
+                     end) ↘ PA.
+Proof.
+  elim : A PA / h.
+  - hauto lq:on ctrs:InterpExt.
+  - hauto l:on.
+  - hauto l:on.
+  - hauto l:on ctrs:InterpExt.
+  - move => m h.
+    apply InterpExt_Univ' => //.
+    case : Compare_dec.lt_dec => //.
+  - hauto l:on ctrs:InterpExt.
+  - hauto lq:on ctrs:InterpExt.
+Qed.
+
+Lemma InterpExt_lt_redundant2 i I A PA
+ (h : ⟦ A ⟧ i , (fun j A =>
+                      match Compare_dec.lt_dec j i with
+                     | left h => I j A
+                     | right _ => False
+                     end) ↘ PA) :
+  ⟦ A ⟧ i , I ↘ PA.
+Proof.
+  elim : A PA / h.
+  - hauto lq:on ctrs:InterpExt.
+  - hauto l:on.
+  - hauto l:on.
+  - hauto l:on ctrs:InterpExt.
+  - move => m ?.
+    apply InterpExt_Univ' => //.
+    case : Compare_dec.lt_dec => //.
+  - hauto l:on ctrs:InterpExt.
+  - hauto lq:on ctrs:InterpExt.
+Qed.
+
+Lemma InterpUnivN_nolt i :
+  InterpUnivN i = InterpExt i (fun j A => exists PA, ⟦ A ⟧ j ↘ PA).
+Proof.
+  simp InterpUnivN.
+  fext => A P.
+  apply propositional_extensionality.
+  hauto l:on use:InterpExt_lt_redundant, InterpExt_lt_redundant2.
+Qed.
+
+#[export]Hint Rewrite InterpUnivN_nolt : InterpUniv.
+
+Lemma InterpExt_Fun_inv i I A B P
+  (h :  ⟦ tPi A B ⟧ i , I ↘ P) :
+  exists (PA : tm -> Prop) (PF : tm -> (tm -> Prop) -> Prop),
+     ⟦ A ⟧ i , I ↘ PA /\
+    (forall a, PA a -> exists PB, PF a PB) /\
+    (forall a PB, PF a PB -> ⟦ B[a..] ⟧ i , I ↘ PB) /\
+    P = ProdSpace PA PF.
+Proof.
+  move E : (tPi A B) h => T h.
+  move : A B E.
+  elim : T P / h => //.
+  - hauto q:on inv:tm.
+  - hauto l:on.
+  - move => *; subst.
+    hauto lq:on inv:Par ctrs:InterpExt use:Par_subst.
+Qed.
+
+
+(* For all of the proofs about InterpUnivN below, we need to
+   do them in two steps. Once for InterpExt, and then tie the
+   knot for the full definition. *)
+
+(* -----  I-PiAlt is admissible (free of PF, the relation R on paper)  ---- *)
+
+
+Lemma InterpExt_Fun_nopf i I A B PA  :
+  ⟦ A ⟧ i , I ↘ PA ->
+  (forall a, PA a -> exists PB, ⟦ B[a..] ⟧ i , I ↘  PB) ->
+  ⟦ tPi A B ⟧ i , I ↘ (ProdSpace PA (fun a PB => ⟦ B[a..] ⟧ i , I ↘ PB)).
+Proof.
+  move => h0 h1. apply InterpExt_Fun =>//.
+Qed.
+
+Lemma InterpUnivN_Fun_nopf i A B PA :
+  ⟦ A ⟧ i ↘ PA ->
+  (forall a, PA a -> exists PB, ⟦ B[a..] ⟧ i ↘ PB) ->
+  ⟦ tPi A B ⟧ i ↘ (ProdSpace PA (fun a PB => ⟦ B[a..] ⟧ i ↘ PB)).
+Proof.
+  hauto l:on use:InterpExt_Fun_nopf rew:db:InterpUniv.
+Qed.
+
+(* --------------- relation is cumulative ----------------- *)
+
+
+Lemma InterpExt_cumulative i j I A PA :
+  i < j ->
+   ⟦ A ⟧ i , I ↘ PA ->
+   ⟦ A ⟧ j , I ↘ PA.
+Proof.
+  move => h h0.
+  elim : A PA /h0;
+    hauto l:on ctrs:InterpExt use:PeanoNat.Nat.lt_trans.
+Qed.
+
+Lemma InterpUnivN_cumulative i A PA :
+   ⟦ A ⟧ i ↘ PA -> forall j, i < j ->
+   ⟦ A ⟧ j ↘ PA.
+Proof.
+  hauto l:on rew:db:InterpUniv use:InterpExt_cumulative.
+Qed.
+
+(* ------------------------------------------------------- *)
+
+(* The logical relation is closed under parallel reduction,
+   forwards and backwards. *)
+
+Lemma InterpExt_preservation i I A B P (h : ⟦ A ⟧ i , I ↘ P) :
+  (A ⇒ B) ->
+  ⟦ B ⟧ i , I ↘ P.
 Proof.
   move : B.
   elim : A P / h; auto.
-  - eauto with iext nfne.
+  - hauto lq:on ctrs:InterpExt db:nfne.
   - hauto lq:on inv:Par ctrs:InterpExt.
   - hauto lq:on inv:Par ctrs:InterpExt.
   - move => A B PA PF hPA ihPA hPB hPB' ihPB T hT.
-    elim /Par_inv : hT=>// ? A0 A1 B0 B1 ? ? [] *; subst.
-    apply InterpExt_Fun; eauto with nfne.
-    eauto using par_cong, Par_refl.
+    elim /Par_inv :  hT => //.
+    move => hPar A0 A1 B0 B1 h0 h1 [? ?] ?; subst.
+    apply InterpExt_Fun; auto.
+    move => a PB hPB0.
+    apply : ihPB; eauto.
+    sfirstorder use:Par_cong, Par_refl.
   - hauto lq:on inv:Par ctrs:InterpExt.
-  - move => a b A ?  ? ? B.
+  - move => a b A  ? ? ? B.
     elim /Par_inv=>// h ? ? ? a0 b0 A0 ? ? ? [] *. subst.
     apply InterpExt_Eq'; eauto with nfne.
-    (* Should have one goal remaining *)
-    rewrite /SEq.
-    fext => p. do 2 f_equal.
+    fext => p.
+    f_equal.
     apply propositional_extensionality.
     hauto lq:on use:Par_Coherent, Coherent_transitive, Coherent_symmetric.
   - move => A B P h0 h1 ih1 C hC.
-    have [D [h2 h3]] := par_confluent _ _ _ h0 hC.
+    have [D [h2 h3]] := Par_confluent _ _ _ h0 hC.
     hauto lq:on ctrs:InterpExt.
 Qed.
 
-Lemma InterpUnivN_preservation n A B P (h : InterpUnivN n A P) :
-  Par A B ->
-  InterpUnivN n B P.
+
+Lemma InterpUnivN_preservation i A B P (h : ⟦ A ⟧ i ↘ P) :
+  (A ⇒ B) ->
+  ⟦ B ⟧ i ↘ P.
 Proof. hauto l:on rew:db:InterpUnivN use: InterpExt_preservation. Qed.
 
-Lemma InterpExt_back_preservation_star i I A B P (h : InterpExt i I B P) :
-  Pars A B ->
-  InterpExt i I A P.
+Lemma InterpExt_back_preservation_star i I A B P (h : ⟦ B ⟧ i , I ↘ P) :
+  A ⇒* B ->
+  ⟦ A ⟧ i , I ↘ P.
 Proof. induction 1; hauto l:on ctrs:InterpExt. Qed.
 
-Lemma InterpExt_preservation_star n I A B P (h : InterpExt n I A P) :
-  Pars A B ->
-  InterpExt n I B P.
+Lemma InterpExt_preservation_star i I A B P (h : ⟦ A ⟧ i , I ↘ P) :
+  A ⇒* B ->
+  ⟦ B ⟧ i , I ↘ P.
 Proof. induction 1; hauto l:on use:InterpExt_preservation. Qed.
 
-Lemma InterpUnivN_preservation_star n A B P (h : InterpUnivN n A P) :
-  Pars A B ->
-  InterpUnivN n B P.
+Lemma InterpUnivN_preservation_star i A B P (h : ⟦ A ⟧ i ↘ P) :
+  A ⇒* B ->
+  ⟦ B ⟧ i ↘ P.
 Proof. hauto l:on rew:db:InterpUnivN use:InterpExt_preservation_star. Qed.
 
-Lemma InterpUnivN_back_preservation_star n A B P (h : InterpUnivN n B P) :
-  Pars A B ->
-  InterpUnivN n A P.
+Lemma InterpUnivN_back_preservation_star i A B P (h : ⟦ B ⟧ i ↘ P) :
+  A ⇒* B ->
+  ⟦ A ⟧ i ↘ P.
 Proof. hauto l:on rew:db:InterpUnivN use:InterpExt_back_preservation_star. Qed.
 
-Lemma InterpUnivN_Coherent n A B P (h : InterpUnivN n B P) :
+(* ---------------------------------------------------------- *)
+
+Lemma InterpUnivN_Coherent i A B P (h : ⟦ B ⟧ i ↘ P) :
   Coherent A B ->
-  InterpUnivN n A P.
+  ⟦ A ⟧ i ↘ P.
 Proof.
   hauto l:on unfold:Coherent use:InterpUnivN_back_preservation_star, InterpUnivN_preservation_star.
 Qed.
 
-Lemma InterpExt_Bool_inv n I P :
-  InterpExt n I tBool P ->
-  P = SBool.
-Proof.
-  move E : tBool => A h.
-  move : E.
-  elim : A P / h=> //; hauto q:on inv:tm,Par.
-Qed.
+(* ---------------------------------------------------------- *)
+(* inversion lemmas for InterpExt. To invert the InterpExt
+   judgment, we have to be careful about the step case. *)
 
-Lemma InterpExt_Ne_inv n I A P :
+Lemma InterpExt_Ne_inv i I A P :
   ne A ->
-  InterpExt n I A P ->
+  ⟦ A ⟧ i , I ↘ P ->
   P = wne.
 Proof.
   move => + h0.
@@ -197,84 +265,72 @@ Proof.
   hauto l:on inv:- db:nfne.
 Qed.
 
-Lemma InterpExt_Void_inv n I P :
-  InterpExt n I tVoid P ->
+Lemma InterpExt_Bool_inv i I P :
+  ⟦ tBool ⟧ i , I ↘ P ->
+  P = fun a => exists v, a ⇒* v /\ (is_bool_val v \/ ne v).
+Proof.
+  move E : tBool => A h.
+  move : E.
+  elim : A P / h; hauto q:on inv:tm,Par.
+Qed.
+
+Lemma InterpExt_Void_inv i I P :
+  ⟦ tVoid ⟧ i , I ↘ P ->
   P = wne.
 Proof.
   move E : tVoid => A h.
   move : E.
-  elim : A P / h; hauto q:on inv:Par,tm.
+  elim : A P / h; hauto lq:on inv:Par.
 Qed.
 
-Lemma InterpExt_Univ_inv n I P m :
-  InterpExt n I (tUniv m) P ->
-  P = SUniv I m /\ m < n.
+Lemma InterpExt_Univ_inv i I P j :
+  ⟦ tUniv j ⟧ i , I ↘ P ->
+  P = I j /\ j < i.
 Proof.
-  move E : (tUniv m) => A h.
+  move E : (tUniv j) => A h.
   move : E.
-  elim : A P / h; hauto q:on inv:Par, tm.
+  elim : A P / h; hauto q:on rew:off inv:Par,tm.
 Qed.
 
-Lemma InterpUnivN_Bool_inv n P :
-  InterpUnivN n tBool P ->
-  P = SBool.
+Lemma InterpUnivN_Bool_inv i P :
+  ⟦ tBool ⟧ i ↘ P ->
+  P = fun a => exists v, a ⇒* v /\ (is_bool_val v \/ ne v).
 Proof. hauto l:on rew:db:InterpUnivN use:InterpExt_Bool_inv. Qed.
 
-Lemma InterpExt_Eq_inv n I a b A P :
-  InterpExt n I (tEq a b A) P ->
-  P = SEq a b /\ wn a /\ wn b /\ wn A.
+
+Lemma InterpExt_Eq_inv i I a b A P :
+  ⟦ tEq a b A ⟧ i , I ↘ P ->
+  (P = fun A => A ⇒* tRefl /\ Coherent a b \/ wne A) /\ wn a /\ wn b /\ wn A.
 Proof.
   move E : (tEq a b A) => T h.
   move : a b A E.
   elim : T P /h => //.
-  - hauto q:on inv:tm.
-  - hauto lq:on ctrs:rtc.
-  - move => A A0 PA hred hA0 ih a b A1 ?. subst.
-    elim /Par_inv : hred=>//.
-    move => hred ? ? ? a2 b2 A2 ? ? ? [] *;subst.
-    split; last by hauto lq:on rew:off ctrs:rtc.
-    specialize ih with (1 := eq_refl).
-    move : ih => [->] *.
-    fext => A. rewrite /SEq. do 2 f_equal.
-    apply propositional_extensionality.
-    hauto lq:on use:Par_Coherent, Coherent_symmetric, Coherent_transitive.
+  hauto q:on inv:tm.
+  hauto lq:on ctrs:rtc.
+  move => A A0 PA hred hA0 ih a b A1 ?. subst.
+  elim /Par_inv : hred=>//.
+  move => hred ? ? ? a2 b2 A2 ? ? ? [] *;subst.
+  split; last by hauto lq:on rew:off ctrs:rtc.
+  specialize ih with (1 := eq_refl).
+  move : ih => [->] *.
+  fext => A. do 2 f_equal.
+  apply propositional_extensionality.
+  hauto lq:on use:Par_Coherent, Coherent_symmetric, Coherent_transitive.
 Qed.
 
-Lemma wn_pi_inj A B : wn (tPi A B) -> wn A /\ wn B.
+Lemma InterpUnivN_Eq_inv i a b A P :
+  ⟦ tEq a b A ⟧ i ↘ P ->
+  P = (fun p => (p ⇒* tRefl /\ Coherent a b) \/ wne p) /\ wn a /\ wn b /\ wn A.
 Proof.
-  move => [T []].
-  move /pars_pi_inv.
-  move => [A0 [B0 [ ? *]]].
-  hauto q:on ctrs:rtc b:on.
+  simp InterpUniv.
+  hauto l:on use:InterpExt_Eq_inv.
 Qed.
 
-Lemma InterpExt_Fun_inv n Interp A B P  (h : InterpExt n Interp (tPi A B) P) :
-  exists (PA : tm -> Prop) (PF : tm -> (tm -> Prop) -> Prop),
-    InterpExt n Interp A PA /\
-    (forall a, PA a -> exists PB, PF a PB) /\
-    (forall a PB, PF a PB -> InterpExt n Interp (subst_tm (a..) B) PB) /\
-    P = ProdSpace PA PF.
-Proof.
-  move E : (tPi A B) h => T h.
-  move : A B E.
-  elim : T P / h => //.
-  - move => *. by subst.
-  - hauto l:on.
-  - move => A A0 PT hr0 hA0 ih A1 B ?. subst.
-    elim /Par_inv : hr0=>// hr0 A2 A3 B0 B1 ? ?[] *. subst.
-    specialize ih with (1 := eq_refl).
-    move : ih => [PA [PF [hPA [hTot [hRes ?]]] ]]. subst.
-    exists PA, PF. repeat split.
-    by eauto with iext.
-    eauto.
-    move => a PB hPB.
-    have : Par (subst_tm (a..) B) (subst_tm (a..) B1) by sfirstorder use:Par_refl, par_cong.
-    eauto with iext.
-Qed.
+(* ------------- relation is deterministic ---------------- *)
 
-Lemma InterpExt_deterministic n I A PA PB :
-  InterpExt n I A PA ->
-  InterpExt n I A PB ->
+Lemma InterpExt_deterministic i I A PA PB :
+  ⟦ A ⟧ i , I ↘ PA ->
+  ⟦ A ⟧ i , I ↘ PB ->
   PA = PB.
 Proof.
   move => h.
@@ -287,9 +343,7 @@ Proof.
     move /InterpExt_Fun_inv : hP.
     intros (PA0 & PF0 & hPA0 & hPB0 & hPB0' & ?); subst.
     have ? : PA0 = PA by sfirstorder. subst.
-    rewrite /ProdSpace.
-    fext => b. f_equal.
-    fext =>  a PB ha.
+    fext => b a PB ha.
     apply propositional_extensionality.
     hauto lq:on rew:off.
   - hauto lq:on rew:off inv:InterpExt ctrs:InterpExt use:InterpExt_Univ_inv.
@@ -297,127 +351,24 @@ Proof.
   - hauto l:on use:InterpExt_preservation.
 Qed.
 
-Lemma InterpExt_Fun_inv_nopf n I A B P  (h : InterpExt n I (tPi A B) P) :
-  exists (PA : tm -> Prop),
-    InterpExt n I A PA /\
-    (forall a, PA a -> exists PB, InterpExt n I (subst_tm (a..) B) PB) /\
-      P = ProdSpace PA (fun a => InterpExt n I (subst_tm (a..) B)).
-Proof.
-  move /InterpExt_Fun_inv : h. intros (PA & PF & hPA & hPF & hPF' & ?); subst.
-  exists PA. repeat split => //.
-  - sfirstorder.
-  - fext => b. rewrite /ProdSpace. f_equal. fext => a PB ha.
-    apply propositional_extensionality.
-    split.
-    + move  : hPF ha . move /[apply]. intros (PB0 & hPB0). move => *.
-      have ? : PB0 = PB by eauto using InterpExt_deterministic. sfirstorder.
-    + sfirstorder.
-Qed.
-
-Lemma InterpUnivN_deterministic n A PA PB :
-  InterpUnivN n A PA ->
-  InterpUnivN n A PB ->
+Lemma InterpUnivN_deterministic i A PA PB :
+  ⟦ A ⟧ i ↘ PA ->
+  ⟦ A ⟧ i ↘ PB ->
   PA = PB.
 Proof.
-  simp InterpUnivN.
-  eauto using InterpExt_deterministic.
+  simp InterpUnivN. apply InterpExt_deterministic.
 Qed.
 
-Lemma InterpExt_cumulative n m I A PA :
-  n < m ->
-  InterpExt n I A PA ->
-  InterpExt m I A PA.
-Proof.
-  move => h h0.
-  elim : A PA /h0;
-    hauto l:on ctrs:InterpExt use:PeanoNat.Nat.lt_trans.
-Qed.
+(* slight generalization to work with any levels using cumulativity. *)
 
-Lemma InterpExt_lt_redundant n I A PA
-  (h : InterpExt n I A PA) :
-      InterpExt n (fun m A PA =>
-                     match Compare_dec.lt_dec m n with
-                     | left h => I m A PA
-                     | right _ => False
-                     end) A PA.
-Proof.
-  elim : A PA / h.
-  - hauto lq:on ctrs:InterpExt.
-  - hauto l:on.
-  - hauto l:on.
-  - hauto l:on ctrs:InterpExt.
-  - move => m h.
-    apply InterpExt_Univ' => //.
-    rewrite /SUniv.
-    case : Compare_dec.lt_dec => //.
-  - hauto l:on ctrs:InterpExt.
-  - hauto lq:on ctrs:InterpExt.
-Qed.
 
-Lemma InterpExt_lt_redundant2 n (I :fin -> tm -> (tm -> Prop) -> Prop ) A PA
-  (h : InterpExt n (fun m A PA =>
-                      match Compare_dec.lt_dec m n with
-                     | left h => I m A PA
-                     | right _ => False
-                     end) A PA) :
-  InterpExt n I A PA.
-Proof.
-  elim : A PA / h.
-  - hauto lq:on ctrs:InterpExt.
-  - hauto l:on.
-  - hauto l:on.
-  - hauto l:on ctrs:InterpExt.
-  - move => m ?.
-    apply InterpExt_Univ' => //.
-    rewrite /SUniv.
-    case : Compare_dec.lt_dec => //.
-  - hauto l:on ctrs:InterpExt.
-  - hauto lq:on ctrs:InterpExt.
-Qed.
-
-Lemma InterpUnivN_nolt n :
-  InterpUnivN n = InterpExt n InterpUnivN.
-Proof.
-  simp InterpUnivN.
-  fext => A P.
-  apply propositional_extensionality.
-  hauto l:on use:InterpExt_lt_redundant, InterpExt_lt_redundant2.
-Qed.
-
-#[export]Hint Rewrite InterpUnivN_nolt : InterpUniv.
-
-Lemma InterpExt_Fun_nopf n I A B PA  :
-  InterpExt n I A PA ->
-  (forall a, PA a -> exists PB, InterpExt n I (subst_tm (a..) B) PB) ->
-  InterpExt n I (tPi A B) (ProdSpace PA (fun a => InterpExt n I (subst_tm (a..) B))).
-Proof.
-  move => h0 h1. apply InterpExt_Fun =>//.
-Qed.
-
-Lemma InterpUnivN_Fun n A B PA :
-  InterpUnivN n A PA ->
-  (forall a, PA a -> exists PB, InterpUnivN n (subst_tm (a..) B) PB) ->
-  InterpUnivN n (tPi A B) (ProdSpace PA (fun a => InterpUnivN n (subst_tm (a..) B))).
-Proof.
-  hauto l:on use:InterpExt_Fun_nopf rew:db:InterpUniv.
-Qed.
-
-Lemma InterpUnivN_Fun_inv_nopf n A B P  (h : InterpUnivN n (tPi A B) P) :
-  exists (PA : tm -> Prop),
-    InterpUnivN n A PA /\
-    (forall a, PA a -> exists PB, InterpUnivN n (subst_tm (a..) B) PB) /\
-      P = ProdSpace PA (fun a => InterpUnivN n (subst_tm (a..) B)).
-Proof.
-  qauto use:InterpExt_Fun_inv_nopf l:on rew:db:InterpUniv.
-Qed.
-
-Lemma InterpExt_deterministic' n m I A PA PB :
-  InterpExt n I A PA ->
-  InterpExt m I A PB ->
+Lemma InterpExt_deterministic' i j I A PA PB :
+   ⟦ A ⟧ i , I ↘ PA ->
+   ⟦ A ⟧ j , I ↘ PB ->
   PA = PB.
 Proof.
   move => h0 h1.
-  case : (Coq.Arith.Compare_dec.lt_eq_lt_dec m n); first case.
+  case : (Coq.Arith.Compare_dec.lt_eq_lt_dec i j); first case.
   - hauto l:on use:InterpExt_cumulative, InterpExt_deterministic.
   - move => *; subst.
     sfirstorder use:InterpExt_deterministic.
@@ -426,53 +377,79 @@ Proof.
     hauto l:on use:InterpExt_cumulative, InterpExt_deterministic.
 Qed.
 
-Lemma InterpUnivN_cumulative n A PA :
-  InterpUnivN n A PA -> forall m, n < m ->
-  InterpUnivN m A PA.
-Proof.
-  hauto l:on rew:db:InterpUniv use:InterpExt_cumulative.
-Qed.
-
-Lemma InterpUnivN_deterministic' n m  A PA PB :
-  InterpUnivN n A PA ->
-  InterpUnivN m A PB ->
+Lemma InterpUnivN_deterministic' i j  A PA PB :
+  ⟦ A ⟧ i ↘ PA ->
+  ⟦ A ⟧ j ↘ PB ->
   PA = PB.
 Proof. hauto lq:on rew:off use:InterpExt_deterministic' rew:db:InterpUniv. Qed.
 
-Lemma InterpExt_back_clos n (I : nat -> tm -> (tm -> Prop) -> Prop) A PA
-  (hI : forall m, m < n -> forall a b, Par a b -> forall PA, I m b PA -> I m a PA ):
-  InterpExt n I A PA ->
-  forall a b, Par a b ->
-         PA b -> PA a.
+(* ----- Improved inversion lemma for functions (Pi Inv Alt) ---------- *)
+
+
+Lemma InterpExt_Fun_inv_nopf i I A B P  (h : InterpExt i I (tPi A B) P) :
+  exists (PA : tm -> Prop),
+     ⟦ A ⟧ i , I ↘ PA /\
+    (forall a, PA a -> exists PB, ⟦ B[a..] ⟧ i , I ↘ PB) /\
+      P = ProdSpace PA (fun a PB => ⟦ B[a..] ⟧ i , I ↘ PB).
 Proof.
-  move => h.
-  elim : A PA / h.
+  move /InterpExt_Fun_inv : h. intros (PA & PF & hPA & hPF & hPF' & ?); subst.
+  exists PA. repeat split => //.
+  - sfirstorder.
+  - fext => b a PB ha.
+    apply propositional_extensionality.
+    split.
+    + move  : hPF ha . move /[apply]. intros (PB0 & hPB0). move => *.
+      have ? : PB0 = PB by eauto using InterpExt_deterministic. sfirstorder.
+    + sfirstorder.
+Qed.
+
+
+Lemma InterpUnivN_Fun_inv_nopf i A B P  (h : InterpUnivN i (tPi A B) P) :
+  exists (PA : tm -> Prop),
+    ⟦ A ⟧ i ↘ PA /\
+    (forall a, PA a -> exists PB, ⟦ B[a..] ⟧ i ↘ PB) /\
+      P = ProdSpace PA (fun a PB => ⟦ B[a..] ⟧ i ↘ PB).
+Proof.
+  qauto use:InterpExt_Fun_inv_nopf l:on rew:db:InterpUniv.
+Qed.
+
+(* ---- Alternative intro rule for Eq ----------- *)
+Lemma InterpUnivN_Eq i a b A:
+  wn a -> wn b -> wn A ->
+  ⟦ tEq a b A ⟧ i ↘ (fun p => (p ⇒* tRefl /\ Coherent a b) \/ wne p).
+Proof.
+  move => [va [? ?]] [vb [? ?]] [vA [? ?]].
+  have ? : InterpUnivN i (tEq va vb vA) (fun p => (p ⇒* tRefl /\ Coherent va vb) \/ wne p)
+    by hauto lq:on ctrs:InterpExt rew:db:InterpUniv.
+  have ? : (tEq a b A) ⇒* (tEq va vb vA) by auto using S_Eq.
+  have : InterpUnivN i (tEq a b A) (fun p => (p ⇒* tRefl /\ Coherent va vb) \/ wne p) by eauto using InterpUnivN_back_preservation_star.
+  move /[dup] /InterpUnivN_Eq_inv. move => [?]. congruence.
+Qed.
+
+
+(* ----  Backward closure for the interpreted sets ----- *)
+Lemma InterpUnivN_back_clos i A PA :
+    ⟦ A ⟧ i ↘ PA ->
+    forall a b, (a ⇒ b) ->
+           PA b -> PA a.
+Proof.
+  simp InterpUniv => h.
+  elim : A PA /h.
   - hauto lq:on ctrs:rtc.
   - hauto lq:on ctrs:rtc.
   - hauto lq:on ctrs:rtc.
   - move => A B PA PF hPA ihA hPFTot hPF ihPF b0 b1 hb01.
-    rewrite /ProdSpace.
-    move => hPB a PB ha hPFa.
-    have ? : Par (tApp b0 a)(tApp b1 a) by hauto lq:on ctrs:Par use:Par_refl.
+    rewrite /ProdSpace => hPB a PB ha hPFa.
+    have ? : (tApp b0 a ⇒ tApp b1 a) by hauto lq:on ctrs:Par use:Par_refl.
     hauto lq:on ctrs:Par.
-  - hauto lq:on.
+  - qauto l:on rew:db:InterpUniv ctrs:InterpExt.
   - hauto lq:on ctrs:rtc.
   - sfirstorder.
 Qed.
 
-Lemma InterpUnivN_back_clos n A PA :
-    InterpUnivN n A PA ->
-    forall a b, Par a b ->
-           PA b -> PA a.
-Proof.
-  simp InterpUniv.
-  apply InterpExt_back_clos.
-  qauto l:on rew:db:InterpUniv ctrs:InterpExt.
-Qed.
-
-Lemma InterpUnivN_back_clos_star n A PA :
-    InterpUnivN n A PA ->
-    forall a b, Pars a b ->
+Lemma InterpUnivN_back_clos_star i A PA :
+    ⟦ A ⟧ i ↘ PA ->
+    forall a b, a ⇒* b ->
            PA b -> PA a.
 Proof.
   move => h a b.
@@ -481,88 +458,76 @@ Qed.
 
 Lemma InterpUnivN_Univ_inv i j :
   j < i ->
-  InterpUnivN i (tUniv j) (fun A : tm => exists (PA : tm -> Prop), InterpUnivN j A PA).
+  ⟦ tUniv j ⟧ i ↘  (fun A : tm => exists (PA : tm -> Prop), InterpUnivN j A PA).
 Proof.
   move => hji.
   simp InterpUniv.
   apply InterpExt_Univ' => [|//].
-  rewrite /SUniv.
   by simp InterpUniv.
 Qed.
 
-Lemma InterpUnivN_Eq_inv n a b A P :
-  InterpUnivN n (tEq a b A) P ->
-  P = SEq a b /\ wn a /\ wn b /\ wn A.
-Proof.
-  simp InterpUniv.
-  hauto l:on use:InterpExt_Eq_inv.
-Qed.
-
 Lemma InterpUnivN_Univ_inv' i j P :
-  InterpUnivN i (tUniv j) P ->
+  ⟦ tUniv j ⟧ i ↘ P ->
   P = (fun A : tm => exists (PA : tm -> Prop), InterpUnivN j A PA) /\ j < i.
 Proof.
-  hauto q:on rew:db:InterpUniv use:InterpExt_Univ_inv unfold:SUniv.
+  hauto q:on rew:db:InterpUniv use:InterpExt_Univ_inv.
 Qed.
 
-Lemma InterpExt_WNe n I A : wne A -> InterpExt n I A wne.
-Proof.
-  rewrite /wne.
-  move => [B [h0]].
-  elim : A B / h0; eauto with iext.
-Qed.
+(* ------------------------ adequacy ------------------------------- *)
 
-Lemma InterpUniv_wn_ty n A PA
-  (h : InterpUnivN n A PA) :
-  wn A.
-Proof.
-  move : n A PA h.
-  elim /Wf_nat.lt_wf_ind => n ih A PA /[dup] hPA.
-  simp InterpUniv.
-  apply InterpExt_wn_ty.
-  move => m /[dup] ?.
-  move : ih. move/[apply] => ih.
-  split.
-  - sfirstorder.
-  - rewrite /SUniv.
-    simp InterpUniv.
-    hauto l:on use:InterpExt_WNe.
-Qed.
+(* P identifies a set of "reducibility candidates" *)
+Definition CR (P : tm -> Prop) :=
+  (forall a, P a -> wn a) /\
+    (forall a, wne a -> P a).
 
-Lemma InterpUniv_adequacy n A PA
-  (h : InterpUnivN n A PA)  :
+(* Every interpretation of types is a reducibility candidate *)
+Lemma adequacy i A PA
+  (h :  ⟦ A ⟧ i ↘ PA) :
   CR PA.
 Proof.
-  move : h.
-  simp InterpUniv.
-  apply adequacy.
-  move => m ?.
-  split.
-  - hauto l:on use:InterpUniv_wn_ty unfold:SUniv.
-  - rewrite /SUniv.
-    move => A0 ?.
-    simp InterpUniv.
-    hauto lq:on use:InterpExt_WNe.
+  elim /Wf_nat.lt_wf_ind : i A PA h.
+  move => i ihn A PA h.
+  simp  InterpUniv in h.
+  elim : A PA / h =>//.
+  - firstorder with nfne.
+  - firstorder with nfne.
+  - hauto q:on db:nfne.
+  - move => A B PA PF hA ihA hTot hRes ih.
+    split.
+    + rewrite /ProdSpace => b hb.
+      have hzero : PA (var_tm var_zero) by hauto lq:on ctrs:rtc.
+      move : hTot (hzero); move/[apply]. move => [PB ?].
+      apply ext_wn with (i := var_zero).
+      hauto q:on.
+    + rewrite /ProdSpace => b wneb a PB ha hPB.
+      suff : wn a by hauto q:on use:wne_app. firstorder.
+  - move => m hlt.
+    split.
+    + move => A [PA h].
+      simp InterpUniv in h.
+      elim : A PA / h; auto with nfne.
+      * move => A B PA PF hPA wnA hTot hRes ih.
+        apply wn_pi; first by auto.
+        have ? : CR PA by hauto lq:on rew:db:InterpUniv.
+        have hzero : PA (var_tm var_zero) by hauto q:on ctrs:rtc.
+        move : hTot (hzero); move/[apply]. move => [PB].
+        move /ih.
+        match goal with [|- wn ?Q -> _] => replace Q with (ren_tm (var_zero..) B) end.
+        eauto using wn_antirenaming.
+        substify. by asimpl.
+      * hauto lq:on use:wn_eq ctrs:rtc.
+      * hauto lq:on ctrs:rtc.
+    + hauto lq:on ctrs:InterpExt use:InterpExt_back_preservation_star rew:db:InterpUniv unfold:wne.
+  - hauto lq:on db:nfne.
 Qed.
 
-Lemma InterpUniv_wn n A PA
-  (h : InterpUnivN n A PA) :
-  forall a, PA a -> wn a.
-Proof. hauto q:on use:InterpUniv_adequacy unfold:wn. Qed.
-
-Lemma InterpUniv_wne n A PA
-  (h : InterpUnivN n A PA) :
-  forall a, wne a -> PA a.
-Proof. hauto q:on use:InterpUniv_adequacy unfold:wn. Qed.
-
-Lemma InterpUnivN_Eq n a b A:
-  wn a -> wn b -> wn A ->
-  InterpUnivN n (tEq a b A) (SEq a b).
+Corollary InterpUniv_wn_ty i A PA
+  (h : ⟦ A ⟧ i ↘ PA) :
+  wn A.
 Proof.
-  move => [va [? ?]] [vb [? ?]] [vA [? ?]].
-  have ? : InterpUnivN n (tEq va vb vA) (SEq va vb)
-    by hauto lq:on ctrs:InterpExt rew:db:InterpUniv.
-  have ? : Pars (tEq a b A) (tEq va vb vA) by auto using S_Eq.
-  have : InterpUnivN n (tEq a b A) (SEq va vb) by eauto using InterpUnivN_back_preservation_star.
-  move /[dup] /InterpUnivN_Eq_inv. move => [?]. congruence.
+  suff : exists PA,  ⟦ tUniv i ⟧ (S i) ↘  PA /\ PA A by hauto q:on use:adequacy.
+  eexists.
+  split.
+  qauto l:on ctrs:InterpExt rew:db:InterpUniv.
+  move =>//. eauto.
 Qed.
