imports.v
@@ -1,9 +1,17 @@
 From Coq Require Export ssreflect ssrbool.
+From Coq Require Export Wf_nat (well_founded_ltof, induction_ltof1).
 From Coq Require Export Logic.PropExtensionality
-  (propositional_extensionality) Program.Basics (const).
+  (propositional_extensionality) Program.Basics (const) FunInd.
 From Equations Require Export Equations.
 From Hammer Require Export Tactics.
-From stdpp Require Export relations (rtc, rtc_transitive, rtc_once, rtc_inv, rtc(..), diamond, confluent, diamond_confluent) option (from_option).
-From Coq Require Export Wf_nat (well_founded_ltof, induction_ltof1).
+From stdpp Require Export relations (rtc, rtc_transitive, rtc_once, rtc_inv, rtc(..), diamond, confluent, diamond_confluent).
 Require Export Psatz.
-From HB Require Export structures.
+
+Global Set Warnings "-notation-overridden".
+From WR Require Export syntax.
+
+Notation "s [ sigmatm ]" := (subst_tm sigmatm s) (at level 7, left associativity) : subst_scope.
+Notation "s ⟨ xitm ⟩" := (ren_tm xitm s) (at level 7, left associativity) : subst_scope.
+Notation "n ∈ 'dom'  Γ " := (n < length Γ) (at level 70, no associativity).
+
+Global Open Scope subst_scope.
