typing.v
@@ -1,99 +1,107 @@
-From WR Require Import syntax join common.
+From WR Require Import imports join common.
 
-(* #[export]Hint Unfold dep_ith : core. *)
-Inductive Wt (Γ : context) : tm -> tm -> Prop :=
-| T_Var i :
-  Wff Γ ->
-  i < length Γ ->
+Reserved Notation "Γ ⊢ a ∈ A" (at level 70).
+Reserved Notation "⊢ Γ" (at level 70).
+
+Inductive Wt : context -> tm -> tm -> Prop :=
+| T_Var Γ i A :
+  ⊢ Γ ->
+  lookup i Γ A ->
   (* ------ *)
-  Wt Γ (var_tm i) (dep_ith Γ i)
+  Γ ⊢ (var_tm i) ∈ A
 
-| T_Void i :
-  Wff Γ ->
+| T_Void Γ i :
+  ⊢ Γ ->
   (* -------- *)
-  Wt Γ tVoid (tUniv i)
+  Γ ⊢ tVoid ∈ (tUniv i)
 
-| T_Pi i A B :
-  Wt Γ A (tUniv i) ->
-  Wt (A :: Γ) B (tUniv i) ->
+| T_Pi Γ i A B :
+  Γ ⊢ A ∈ (tUniv i) ->
+  (A :: Γ) ⊢ B ∈ (tUniv i) ->
   (* --------------------- *)
-  Wt Γ (tPi A B) (tUniv i)
+  Γ ⊢ (tPi A B) ∈ (tUniv i)
 
-| T_Abs A a B i :
-  Wt Γ (tPi A B) (tUniv i) ->
-  Wt (A :: Γ) a B ->
+| T_Abs Γ A a B i :
+  Γ ⊢ (tPi A B) ∈ (tUniv i) ->
+  (A :: Γ) ⊢ a ∈ B ->
   (* -------------------- *)
-  Wt Γ (tAbs a) (tPi A B)
+  Γ ⊢ (tAbs a) ∈ (tPi A B)
 
-| T_App a A B b :
-  Wt Γ a (tPi A B) ->
-  Wt Γ b A ->
+| T_App Γ a A B b :
+  Γ ⊢ a ∈ (tPi A B) ->
+  Γ ⊢ b ∈ A ->
   (* -------------------- *)
-  Wt Γ (tApp a b) (subst_tm (b..) B)
+  Γ ⊢ (tApp a b) ∈ (B [ b.. ])
 
-| T_Conv a A B i :
-  Wt Γ a A ->
-  Wt Γ B (tUniv i) ->
+| T_Conv Γ a A B i :
+  Γ ⊢ a ∈ A ->
+  Γ ⊢ B ∈ (tUniv i) ->
   Coherent A B ->
   (* ----------- *)
-  Wt Γ a B
+  Γ ⊢ a ∈ B
 
-| T_True :
-  Wff Γ ->
+| T_True Γ :
+  ⊢ Γ ->
   (* --------- *)
-  Wt Γ tTrue tBool
+  Γ ⊢ tTrue ∈ tBool
 
-| T_False :
-  Wff Γ ->
+| T_False Γ :
+  ⊢ Γ ->
   (* --------- *)
-  Wt Γ tFalse tBool
+  Γ ⊢ tFalse ∈ tBool
 
-| T_If a b c A :
-  Wt Γ a tBool ->
-  Wt Γ b A ->
-  Wt Γ c A ->
+| T_If Γ a b c A i :
+  (tBool :: Γ) ⊢ A ∈ (tUniv i) ->
+  Γ ⊢ a ∈ tBool ->
+  Γ ⊢ b ∈ (A [tTrue..]) ->
+  Γ ⊢ c ∈ (A [tFalse..]) ->
   (* ------------ *)
-  Wt Γ (tIf a b c) A
+  Γ ⊢ (tIf a b c) ∈ (A [a..])
 
-| T_Bool i :
-  Wff Γ ->
+| T_Bool Γ i :
+  ⊢ Γ ->
   (* ----------- *)
-  Wt Γ tBool (tUniv i)
+  Γ ⊢ tBool ∈ (tUniv i)
 
-| T_Univ i j :
-  Wff Γ ->
-  i < j ->
+| T_Univ Γ i :
+  ⊢ Γ ->
   (* ------------ *)
-  Wt Γ (tUniv i) (tUniv j)
+  Γ ⊢ (tUniv i) ∈ (tUniv (S i))
 
-| T_Refl a A:
-  Wff Γ ->
-  Wt Γ a A ->
+| T_Refl Γ a A:
+  ⊢ Γ ->
+  Γ ⊢ a ∈ A ->
   (* ------ *)
-  Wt Γ tRefl (tEq a a A)
+  Γ ⊢ tRefl ∈ (tEq a a A)
 
-| T_Eq a b A i j :
-  Wt Γ a A ->
-  Wt Γ b A ->
-  Wt Γ A (tUniv j) ->
+| T_Eq Γ a b A i j :
+  Γ ⊢ a ∈ A ->
+  Γ ⊢ b ∈ A ->
+  Γ ⊢ A ∈ (tUniv j) ->
   (* ----------------------- *)
-  Wt Γ (tEq a b A) (tUniv i)
+  Γ ⊢ (tEq a b A) ∈ (tUniv i)
 
-| T_J t a b p A i j C : 
-  Wt Γ a A ->
-  Wt Γ b A ->
-  Wt Γ A (tUniv j) ->
-  Wt Γ p (tEq a b A) ->
-  Wt (tEq (ren_tm shift a) (var_tm 0) (ren_tm shift A) :: A :: Γ) C (tUniv i) ->
-  Wt Γ t (subst_tm (tRefl .: a ..) C) ->
-  Wt Γ (tJ t a b p) (subst_tm (p .: b..) C)
-  
+| T_J Γ t a b p A i j C : 
+  Γ ⊢ a ∈  A ->
+  Γ ⊢ b ∈ A ->
+  Γ ⊢ A ∈ (tUniv j) ->
+  Γ ⊢ p ∈ (tEq a b A) ->
+  (tEq (ren_tm shift a) (var_tm 0) (ren_tm shift A) :: A :: Γ) ⊢ C ∈ (tUniv i) ->
+  Γ ⊢ t ∈ (C [tRefl .: a ..]) ->
+  Γ ⊢ (tJ t a b p) ∈ (C [p .: b..])
 
-with Wff (Γ : context) : Prop :=
-| Wff_intro F :
-  (forall i, i < length Γ -> Wt (skipn (S i) Γ) (ith Γ i) (tUniv (F i))) ->
-  (* ---------------------------------------------------------------- *)
-  Wff Γ.
+with Wff : context -> Prop :=
+| Wff_nil :
+(* ----------------- *)
+  ⊢ nil
+| Wff_cons Γ A i :
+  ⊢ Γ ->
+  Γ ⊢ A ∈ tUniv i ->
+(* ----------------- *)
+  ⊢ A :: Γ
+where 
+  "Γ ⊢ a ∈ A" := (Wt Γ a A) and "⊢ Γ" := (Wff Γ).
+
 
 Scheme wt_ind := Induction for Wt Sort Prop
     with wff_ind := Induction for Wff Sort Prop.
